Split ArraySlice.lean and ScalarTac.Lemmas.lean

backends/lean/Aeneas/Std/Slice.lean
@@ -1,180 +1,11 @@
 /- Arrays/Slices -/
-import Lean
-import Lean.Meta.Tactic.Simp
-import Init.Data.List.Basic
-import Mathlib.Tactic.Linarith
 import Aeneas.List
-import Aeneas.Std.Scalar
+import Aeneas.Std.Array.Core
 import Aeneas.Std.Range
-import Aeneas.Std.Core
-import Aeneas.ScalarTac
-import Aeneas.Progress.Core
 
-namespace Aeneas
-
-namespace Std
+namespace Aeneas.Std
 
 open Result Error core.ops.range
-
-/-!
-# Notations for `List`
--/
-instance {α : Type u} : GetElem (List α) Usize α (fun l i => i.val < l.length) where
-  getElem l i h := getElem l i.val h
-
-instance {α : Type u} : GetElem? (List α) Usize α (fun l i => i < l.length) where
-  getElem? l i := getElem? l i.val
-
-/-!
-# Array
--/
-
-def Array (α : Type u) (n : Usize) := { l : List α // l.length = n.val }
-
-/-- We need this to coerce arrays to lists without marking `Array` as reducible.
-    Also not that we *do not* want to mark `Array` as reducible: it triggers issues.
--/
-instance (α : Type u) (n : Usize) : CoeOut (Array α n) (List α) where
-  coe := λ v => v.val
-
-instance [BEq α] : BEq (Array α n) := SubtypeBEq _
-
-instance [BEq α] [LawfulBEq α] : LawfulBEq (Array α n) := SubtypeLawfulBEq _
-
-/- Registering some theorems for `scalar_tac` -/
-@[scalar_tac a]
-theorem Array.length_eq {α : Type u} {n : Usize} (a : Array α n) : a.val.length = n.val := by
-  cases a; simp[*]
-
--- TODO: move/remove?
-@[scalar_tac a]
-theorem Array.subtype_property {α : Type u} {n : Usize} {p : Array α n → Prop} (a : Subtype p) : p a.val := a.property
-
-@[simp]
-abbrev Array.length {α : Type u} {n : Usize} (v : Array α n) : Nat := v.val.length
-
-@[simp]
-abbrev Array.v {α : Type u} {n : Usize} (v : Array α n) : List α := v.val
-
-example {α: Type u} {n : Usize} (v : Array α n) : v.length ≤ Usize.max := by
-  scalar_tac
-
-def Array.make {α : Type u} (n : Usize) (init : List α) (hl : init.length = n.val := by simp) :
-  Array α n := ⟨ init, by apply hl ⟩
-
-example : Array Int (Usize.ofNat 2) := Array.make (Usize.ofNat 2) [0, 1] (by simp)
-
-example : Array Int (Usize.ofNat 2) :=
-  let x := 0
-  let y := 1
-  Array.make (Usize.ofNat 2) [x, y]
-
-example : Result (Array Int (Usize.ofNat 2)) := do
-  let x ← ok 0
-  let y ← ok 1
-  ok (Array.make (Usize.ofNat 2) [x, y])
-
-@[reducible] instance {α : Type u} {n : Usize} : GetElem (Array α n) Nat α (fun a i => i < a.val.length) where
-  getElem a i h := getElem a.val i h
-
-@[reducible] instance {α : Type u} {n : Usize} : GetElem? (Array α n) Nat α (fun a i => i < a.val.length) where
-  getElem? a i := getElem? a.val i
-
-@[simp, scalar_tac_simp] theorem Array.getElem?_Nat_eq {α : Type u} {n : Usize} (v : Array α n) (i : Nat) : v[i]? = v.val[i]? := by rfl
-@[simp, scalar_tac_simp] theorem Array.getElem!_Nat_eq {α : Type u} [Inhabited α] {n : Usize} (v : Array α n) (i : Nat) : v[i]! = v.val[i]! := by rfl
-
-@[reducible] instance {α : Type u} {n : Usize} : GetElem (Array α n) Usize α (fun a i => i.val < a.val.length) where
-  getElem a i h := getElem a.val i.val h
-
-@[reducible] instance {α : Type u} {n : Usize} : GetElem? (Array α n) Usize α (fun a i => i.val < a.val.length) where
-  getElem? a i := getElem? a.val i.val
-
-@[simp, scalar_tac_simp] theorem Array.getElem?_Usize_eq {α : Type u} {n : Usize} (v : Array α n) (i : Usize) : v[i]? = v.val[i.val]? := by rfl
-@[simp, scalar_tac_simp] theorem Array.getElem!_Usize_eq {α : Type u} [Inhabited α] {n : Usize} (v : Array α n) (i : Usize) : v[i]! = v.val[i.val]! := by rfl
-
-@[simp, scalar_tac_simp] abbrev Array.get? {α : Type u} {n : Usize} (v : Array α n) (i : Nat) : Option α := getElem? v i
-@[simp, scalar_tac_simp] abbrev Array.get! {α : Type u} {n : Usize} [Inhabited α] (v : Array α n) (i : Nat) : α := getElem! v i
-
-@[simp]
-abbrev Array.slice {α : Type u} {n : Usize} [Inhabited α] (v : Array α n) (i j : Nat) : List α :=
-  v.val.slice i j
-
-def Array.index_usize {α : Type u} {n : Usize} (v: Array α n) (i: Usize) : Result α :=
-  match v[i]? with
-  | none => fail .arrayOutOfBounds
-  | some x => ok x
-
--- For initialization
-def Array.repeat {α : Type u} (n : Usize) (x : α) : Array α n :=
-  ⟨ List.replicate n.val x, by simp_all ⟩
-
-@[progress]
-theorem Array.repeat_spec {α : Type u} (n : Usize) (x : α) :
-  ∃ a, Array.repeat n x = a ∧ a.val = List.replicate n.val x := by
-  simp [Array.repeat]
-
-/- In the theorems below: we don't always need the `∃ ..`, but we use one
-   so that `progress` introduces an opaque variable and an equality. This
-   helps control the context.
- -/
-
-@[progress]
-theorem Array.index_usize_spec {α : Type u} {n : Usize} [Inhabited α] (v: Array α n) (i: Usize)
-  (hbound : i.val < v.length) :
-  ∃ x, v.index_usize i = ok x ∧ x = v.val[i.val]! := by
-  simp only [index_usize]
-  simp at *
-  split <;> simp_all
-
-def Array.set {α : Type u} {n : Usize} (v: Array α n) (i: Usize) (x: α) : Array α n :=
-  ⟨ v.val.set i.val x, by have := v.property; simp [*] ⟩
-
-def Array.set_opt {α : Type u} {n : Usize} (v: Array α n) (i: Usize) (x: Option α) : Array α n :=
-  ⟨ v.val.set_opt i.val x, by have := v.property; simp [*] ⟩
-
-@[simp]
-theorem Array.set_val_eq {α : Type u} {n : Usize} (v: Array α n) (i: Usize) (x: α) :
-  (v.set i x).val = v.val.set i.val x := by
-  simp [set]
-
-@[simp]
-theorem Array.set_opt_val_eq {α : Type u} {n : Usize} (v: Array α n) (i: Usize) (x: Option α) :
-  (v.set_opt i x).val = v.val.set_opt i.val x := by
-  simp [set_opt]
-
-@[scalar_tac_simp]
-theorem Array.set_length {α : Type u} {n : Usize} (v: Array α n) (i: Usize) (x: α) :
-  (v.set i x).length = v.length := by simp
-
-def Array.update {α : Type u} {n : Usize} (v: Array α n) (i: Usize) (x: α) : Result (Array α n) :=
-  match v[i]? with
-  | none => fail .arrayOutOfBounds
-  | some _ =>
-    ok ⟨ v.val.set i.val x, by have := v.property; simp [*] ⟩
-
-@[progress]
-theorem Array.update_spec {α : Type u} {n : Usize} (v: Array α n) (i: Usize) (x : α)
-  (hbound : i.val < v.length) :
-  ∃ nv, v.update i x = ok nv ∧
-  nv = v.set i x
-  := by
-  simp only [update, set]
-  simp at *
-  split <;> simp_all
-
-def Array.index_mut_usize {α : Type u} {n : Usize} (v: Array α n) (i: Usize) :
-  Result (α × (α -> Array α n)) := do
-  let x ← index_usize v i
-  ok (x, set v i)
-
-@[progress]
-theorem Array.index_mut_usize_spec {α : Type u} {n : Usize} [Inhabited α] (v: Array α n) (i: Usize)
-  (hbound : i.val < v.length) :
-  ∃ x, v.index_mut_usize i = ok (x, set v i) ∧
-  x = v.val.get! i.val := by
-  simp only [index_mut_usize, Bind.bind, bind]
-  have ⟨ x, h ⟩ := index_usize_spec v i hbound
-  simp [h]
 
 /-!
 # Slice
@@ -315,96 +146,10 @@ theorem Slice.index_mut_usize_spec {α : Type u} [Inhabited α] (v: Slice α) (i
   have ⟨ x, h ⟩ := Slice.index_usize_spec v i hbound
   simp [h]
 
-/- Array to slice/subslices -/
-
-@[progress_pure_def]
-def Array.to_slice {α : Type u} {n : Usize} (v : Array α n) : Slice α :=
-  ⟨ v.val, by scalar_tac ⟩
-
-def Array.from_slice {α : Type u} {n : Usize} (a : Array α n) (s : Slice α) : Array α n :=
-  if h: s.val.length = n.val then
-    ⟨ s.val, by simp [*] ⟩
-  else a -- Unreachable case
-
 @[simp]
-theorem Array.from_slice_val {α : Type u} {n : Usize} (a : Array α n) (ns : Slice α) (h : ns.val.length = n.val) :
-  (from_slice a ns).val = ns.val
-  := by simp [from_slice, *]
-
-@[progress_pure_def]
-def Array.to_slice_mut {α : Type u} {n : Usize} (a : Array α n) :
-  Slice α × (Slice α → Array α n) :=
-  (Array.to_slice a, Array.from_slice a)
-
-def Array.subslice {α : Type u} {n : Usize} (a : Array α n) (r : Range Usize) : Result (Slice α) :=
-  -- TODO: not completely sure here
-  if r.start.val < r.end_.val ∧ r.end_.val ≤ a.val.length then
-    ok ⟨ a.val.slice r.start.val r.end_.val,
-          by
-            have := a.val.slice_length_le r.start.val r.end_.val
-            scalar_tac ⟩
-  else
-    fail panic
-
-@[progress]
-theorem Array.subslice_spec {α : Type u} {n : Usize} [Inhabited α] (a : Array α n) (r : Range Usize)
-  (h0 : r.start.val < r.end_.val) (h1 : r.end_.val ≤ a.val.length) :
-  ∃ s, subslice a r = ok s ∧
-  s.val = a.val.slice r.start.val r.end_.val ∧
-  (∀ i, i + r.start.val < r.end_.val → s.val[i]! = a.val[r.start.val + i]!)
-  := by
-  simp only [subslice, true_and, h0, h1, ↓reduceIte, ok.injEq, exists_eq_left', true_and]
-  intro i _
-  have := List.getElem!_slice r.start.val r.end_.val i a.val (by scalar_tac) (by scalar_tac)
-  simp only [this]
-
-set_option maxHeartbeats 500000
-
-def Array.update_subslice {α : Type u} {n : Usize} (a : Array α n) (r : Range Usize) (s : Slice α) : Result (Array α n) :=
-  -- TODO: not completely sure here
-  if h: r.start.val < r.end_.val ∧ r.end_.val ≤ a.length ∧ s.val.length = r.end_.val - r.start.val then
-    let s_beg := a.val.take r.start.val
-    let s_end := a.val.drop r.end_.val
-    have : s_beg.length = r.start.val := by
-      scalar_tac
-    have : s_end.length = a.val.length - r.end_.val := by
-      scalar_tac
-    let na := s_beg.append (s.val.append s_end)
-    have : na.length = a.val.length:= by
-      simp [na]; scalar_tac
-    ok ⟨ na, by simp_all ⟩
-  else
-    fail panic
-
--- TODO: it is annoying to write `.val` everywhere. We could leverage coercions,
--- but: some symbols like `+` are already overloaded to be notations for monadic
--- operations/
--- We should introduce special symbols for the monadic arithmetic operations
--- (the user will never write those symbols directly).
-@[progress]
-theorem Array.update_subslice_spec {α : Type u} {n : Usize} [Inhabited α] (a : Array α n) (r : Range Usize) (s : Slice α)
-  (_ : r.start.val < r.end_.val) (_ : r.end_.val ≤ a.length) (_ : s.length = r.end_.val - r.start.val) :
-  ∃ na, update_subslice a r s = ok na ∧
-  (∀ i, i < r.start.val → na[i]! = a[i]!) ∧
-  (∀ i, r.start.val ≤ i → i < r.end_.val → na[i]! = s[i - r.start.val]!) ∧
-  (∀ i, r.end_.val ≤ i → i < n.val → na[i]! = a[i]!) := by
-  simp only [update_subslice, length, and_true, true_and, List.append_eq,
-    get!, Slice.get!, ↓reduceDIte, ok.injEq, exists_eq_left', *]
-  have h := List.replace_slice_getElem! r.start.val r.end_.val a.val s.val
-    (by scalar_tac) (by scalar_tac) (by scalar_tac)
-  simp [List.replace_slice] at h
-  have ⟨ h0, h1, h2 ⟩ := h
-  clear h
-  split_conjs
-  . intro i _
-    have := h0 i (by scalar_tac)
-    simp_all
-  . intro i _ _
-    have := h1 i (by scalar_tac) (by scalar_tac)
-    simp [*]
-  . intro i _ _
-    have := h2 i (by scalar_tac) (by scalar_tac)
-    simp [*]
+theorem Slice.update_index_eq α [Inhabited α] (x : Slice α) (i : Usize) :
+  x.set i (x.val[i.val]!) = x := by
+  simp only [Slice, Subtype.eq_iff, set_val_eq, List.set_getElem!]
 
 def Slice.subslice {α : Type u} (s : Slice α) (r : Range Usize) : Result (Slice α) :=
   -- TODO: not completely sure here
@@ -465,17 +210,6 @@ theorem Slice.update_subslice_spec {α : Type u} [Inhabited α] (a : Slice α) (
   . intro i _ _
     have := h2 i (by scalar_tac) (by scalar_tac)
     simp [*]
-
-@[simp]
-theorem Array.set_getElem!_eq α n [Inhabited α] (x : Array α n) (i : Usize) :
-  x.set i (x.val[i.val]!) = x := by
-  have := @List.set_getElem_self _ x.val i.val
-  simp only [Array, Subtype.eq_iff, set_val_eq, List.set_getElem!]
-
-@[simp]
-theorem Slice.update_index_eq α [Inhabited α] (x : Slice α) (i : Usize) :
-  x.set i (x.val[i.val]!) = x := by
-  simp only [Slice, Subtype.eq_iff, set_val_eq, List.set_getElem!]
 
 /- Trait declaration: [core::slice::index::private_slice_index::Sealed] -/
 structure core.slice.index.private_slice_index.Sealed (Self : Type) where
@@ -566,20 +300,6 @@ def core.slice.index.Slice.index_mut
   (s : Slice T) (i : I) : Result (Output × (Output → Slice T)) :=
   inst.index_mut i s
 
-/- [core::array::[T; N]::index]: forward function -/
-def core.array.Array.index
-  {T I Output : Type} {N : Usize} (inst : core.ops.index.Index (Slice T) I Output)
-  (a : Array T N) (i : I) : Result Output :=
-  inst.index a.to_slice i
-
-/- [core::array::[T; N]::index_mut]: forward function -/
-def core.array.Array.index_mut
-  {T I Output : Type} {N : Usize} (inst : core.ops.index.IndexMut (Slice T) I Output)
-  (a : Array T N) (i : I) :
-  Result (Output × (Output → Array T N)) := do
-  let (s, back) ← inst.index_mut a.to_slice i
-  ok (s, fun o => Array.from_slice a (back o))
-
 /- Trait implementation: [core::slice::index::private_slice_index::Sealed<Range<USize>>] -/
 def core.slice.index.private_slice_index.SealedRangeUsizeInst
   : core.slice.index.private_slice_index.Sealed (Range Usize) := {}
@@ -610,21 +330,6 @@ def core.ops.index.IndexMutSliceInst {T I Output : Type}
   core.ops.index.IndexMut (Slice T) I Output := {
   indexInst := core.ops.index.IndexSliceInst inst
   index_mut := core.slice.index.Slice.index_mut inst
-}
-
-/- Trait implementation: [core::array::[T; N]] -/
-def core.ops.index.IndexArrayInst {T I Output : Type} {N : Usize}
-  (inst : core.ops.index.Index (Slice T) I Output) :
-  core.ops.index.Index (Array T N) I Output := {
-  index := core.array.Array.index inst
-}
-
-/- Trait implementation: [core::array::[T; N]] -/
-def core.ops.index.IndexMutArrayInst {T I Output : Type} {N : Usize}
-  (inst : core.ops.index.IndexMut (Slice T) I Output) :
-  core.ops.index.IndexMut (Array T N) I Output := {
-  indexInst := core.ops.index.IndexArrayInst inst.indexInst
-  index_mut := core.array.Array.index_mut inst
 }
 
 /- [core::slice::index::usize::get]: forward function -/
@@ -680,8 +385,6 @@ def core.slice.Slice.copy_from_slice {T : Type} (_ : core.marker.Copy T)
   if s.len = src.len then ok src
   else fail panic
 
-/- [core::array::TryFromSliceError] -/
-def core.array.TryFromSliceError := ()
 
 /- [core::slice::index::{core::slice::index::SliceIndex<@Slice<T>> for core::ops::range::RangeFrom<usize>}::get] -/
 def core.slice.index.SliceIndexRangeFromUsizeSlice.get {T : Type} (r : core.ops.range.RangeFrom Usize) (s : Slice T) : Result (Option (Slice T)) :=
@@ -755,6 +458,4 @@ def core.slice.index.SliceIndexRangeFromUsizeSlice (T : Type) :
     core.slice.index.SliceIndexRangeFromUsizeSlice.index_mut
 }
 
-end Std
-
-end Aeneas
+end Aeneas.Std
