backends/lean/Aeneas/Progress/Core.lean
@@ -166,7 +166,8 @@ def Extension := SimpleScopedEnvExtension (DiscrTreeKey × Name) Rules
 deriving Inhabited
 
 def Rules.insert (r : Rules) (kv : Array DiscrTree.Key × Name) : Rules :=
-  { r with rules := r.rules.insertCore kv.fst kv.snd }
+  { rules := r.rules.insertCore kv.fst kv.snd,
+    deactivated := r.deactivated.erase kv.snd }
 
 def Rules.erase (r : Rules) (k : Name) : Rules :=
   { r with deactivated := r.deactivated.insert k }
