backends/lean/Aeneas/ScalarTac.lean
@@ -1,3 +1,4 @@
 import Aeneas.ScalarTac.ScalarTac
 import Aeneas.ScalarTac.Lemmas
+import Aeneas.ScalarTac.Tests
 import Aeneas.Arith.Lemmas
