backends/lean/Aeneas/Std/Array.lean
@@ -1,0 +1,3 @@
+import Aeneas.Std.Array.Array
+import Aeneas.Std.Array.ArraySlice
+import Aeneas.Std.Array.Core
