backends/lean/Aeneas/Std/Array/Array.lean
@@ -1,0 +1,166 @@
+/- Arrays/Slices -/
+import Aeneas.List
+import Aeneas.Progress.Core
+
+namespace Aeneas.Std
+
+open Result Error
+
+/-!
+# Array
+-/
+
+def Array (α : Type u) (n : Usize) := { l : List α // l.length = n.val }
+
+/-- We need this to coerce arrays to lists without marking `Array` as reducible.
+    Also not that we *do not* want to mark `Array` as reducible: it triggers issues.
+-/
+instance (α : Type u) (n : Usize) : CoeOut (Array α n) (List α) where
+  coe := λ v => v.val
+
+instance [BEq α] : BEq (Array α n) := SubtypeBEq _
+
+instance [BEq α] [LawfulBEq α] : LawfulBEq (Array α n) := SubtypeLawfulBEq _
+
+/- Registering some theorems for `scalar_tac` -/
+@[scalar_tac a]
+theorem Array.length_eq {α : Type u} {n : Usize} (a : Array α n) : a.val.length = n.val := by
+  cases a; simp[*]
+
+-- TODO: move/remove?
+@[scalar_tac a]
+theorem Array.subtype_property {α : Type u} {n : Usize} {p : Array α n → Prop} (a : Subtype p) : p a.val := a.property
+
+@[simp]
+abbrev Array.length {α : Type u} {n : Usize} (v : Array α n) : Nat := v.val.length
+
+@[simp]
+abbrev Array.v {α : Type u} {n : Usize} (v : Array α n) : List α := v.val
+
+example {α: Type u} {n : Usize} (v : Array α n) : v.length ≤ Usize.max := by
+  scalar_tac
+
+def Array.make {α : Type u} (n : Usize) (init : List α) (hl : init.length = n.val := by simp) :
+  Array α n := ⟨ init, by apply hl ⟩
+
+example : Array Int (Usize.ofNat 2) := Array.make (Usize.ofNat 2) [0, 1] (by simp)
+
+example : Array Int (Usize.ofNat 2) :=
+  let x := 0
+  let y := 1
+  Array.make (Usize.ofNat 2) [x, y]
+
+example : Result (Array Int (Usize.ofNat 2)) := do
+  let x ← ok 0
+  let y ← ok 1
+  ok (Array.make (Usize.ofNat 2) [x, y])
+
+@[reducible] instance {α : Type u} {n : Usize} : GetElem (Array α n) Nat α (fun a i => i < a.val.length) where
+  getElem a i h := getElem a.val i h
+
+@[reducible] instance {α : Type u} {n : Usize} : GetElem? (Array α n) Nat α (fun a i => i < a.val.length) where
+  getElem? a i := getElem? a.val i
+
+@[simp, scalar_tac_simp] theorem Array.getElem?_Nat_eq {α : Type u} {n : Usize} (v : Array α n) (i : Nat) : v[i]? = v.val[i]? := by rfl
+@[simp, scalar_tac_simp] theorem Array.getElem!_Nat_eq {α : Type u} [Inhabited α] {n : Usize} (v : Array α n) (i : Nat) : v[i]! = v.val[i]! := by rfl
+
+@[reducible] instance {α : Type u} {n : Usize} : GetElem (Array α n) Usize α (fun a i => i.val < a.val.length) where
+  getElem a i h := getElem a.val i.val h
+
+@[reducible] instance {α : Type u} {n : Usize} : GetElem? (Array α n) Usize α (fun a i => i.val < a.val.length) where
+  getElem? a i := getElem? a.val i.val
+
+@[simp, scalar_tac_simp] theorem Array.getElem?_Usize_eq {α : Type u} {n : Usize} (v : Array α n) (i : Usize) : v[i]? = v.val[i.val]? := by rfl
+@[simp, scalar_tac_simp] theorem Array.getElem!_Usize_eq {α : Type u} [Inhabited α] {n : Usize} (v : Array α n) (i : Usize) : v[i]! = v.val[i.val]! := by rfl
+
+@[simp, scalar_tac_simp] abbrev Array.get? {α : Type u} {n : Usize} (v : Array α n) (i : Nat) : Option α := getElem? v i
+@[simp, scalar_tac_simp] abbrev Array.get! {α : Type u} {n : Usize} [Inhabited α] (v : Array α n) (i : Nat) : α := getElem! v i
+
+@[simp]
+abbrev Array.slice {α : Type u} {n : Usize} [Inhabited α] (v : Array α n) (i j : Nat) : List α :=
+  v.val.slice i j
+
+def Array.index_usize {α : Type u} {n : Usize} (v: Array α n) (i: Usize) : Result α :=
+  match v[i]? with
+  | none => fail .arrayOutOfBounds
+  | some x => ok x
+
+-- For initialization
+def Array.repeat {α : Type u} (n : Usize) (x : α) : Array α n :=
+  ⟨ List.replicate n.val x, by simp_all ⟩
+
+@[progress]
+theorem Array.repeat_spec {α : Type u} (n : Usize) (x : α) :
+  ∃ a, Array.repeat n x = a ∧ a.val = List.replicate n.val x := by
+  simp [Array.repeat]
+
+/- In the theorems below: we don't always need the `∃ ..`, but we use one
+   so that `progress` introduces an opaque variable and an equality. This
+   helps control the context.
+ -/
+
+@[progress]
+theorem Array.index_usize_spec {α : Type u} {n : Usize} [Inhabited α] (v: Array α n) (i: Usize)
+  (hbound : i.val < v.length) :
+  ∃ x, v.index_usize i = ok x ∧ x = v.val[i.val]! := by
+  simp only [index_usize]
+  simp at *
+  split <;> simp_all
+
+def Array.set {α : Type u} {n : Usize} (v: Array α n) (i: Usize) (x: α) : Array α n :=
+  ⟨ v.val.set i.val x, by have := v.property; simp [*] ⟩
+
+def Array.set_opt {α : Type u} {n : Usize} (v: Array α n) (i: Usize) (x: Option α) : Array α n :=
+  ⟨ v.val.set_opt i.val x, by have := v.property; simp [*] ⟩
+
+@[simp]
+theorem Array.set_val_eq {α : Type u} {n : Usize} (v: Array α n) (i: Usize) (x: α) :
+  (v.set i x).val = v.val.set i.val x := by
+  simp [set]
+
+@[simp]
+theorem Array.set_opt_val_eq {α : Type u} {n : Usize} (v: Array α n) (i: Usize) (x: Option α) :
+  (v.set_opt i x).val = v.val.set_opt i.val x := by
+  simp [set_opt]
+
+@[scalar_tac_simp]
+theorem Array.set_length {α : Type u} {n : Usize} (v: Array α n) (i: Usize) (x: α) :
+  (v.set i x).length = v.length := by simp
+
+def Array.update {α : Type u} {n : Usize} (v: Array α n) (i: Usize) (x: α) : Result (Array α n) :=
+  match v[i]? with
+  | none => fail .arrayOutOfBounds
+  | some _ =>
+    ok ⟨ v.val.set i.val x, by have := v.property; simp [*] ⟩
+
+@[progress]
+theorem Array.update_spec {α : Type u} {n : Usize} (v: Array α n) (i: Usize) (x : α)
+  (hbound : i.val < v.length) :
+  ∃ nv, v.update i x = ok nv ∧
+  nv = v.set i x
+  := by
+  simp only [update, set]
+  simp at *
+  split <;> simp_all
+
+def Array.index_mut_usize {α : Type u} {n : Usize} (v: Array α n) (i: Usize) :
+  Result (α × (α -> Array α n)) := do
+  let x ← index_usize v i
+  ok (x, set v i)
+
+@[progress]
+theorem Array.index_mut_usize_spec {α : Type u} {n : Usize} [Inhabited α] (v: Array α n) (i: Usize)
+  (hbound : i.val < v.length) :
+  ∃ x, v.index_mut_usize i = ok (x, set v i) ∧
+  x = v.val.get! i.val := by
+  simp only [index_mut_usize, Bind.bind, bind]
+  have ⟨ x, h ⟩ := index_usize_spec v i hbound
+  simp [h]
+
+@[simp]
+theorem Array.set_getElem!_eq α n [Inhabited α] (x : Array α n) (i : Usize) :
+  x.set i (x.val[i.val]!) = x := by
+  have := @List.set_getElem_self _ x.val i.val
+  simp only [Array, Subtype.eq_iff, set_val_eq, List.set_getElem!]
+
+end Aeneas.Std
